Infer equations from functions involving anonymous fixpoints.

tests/Equation.v
@@ -1,10 +1,14 @@
 Require Import MetaCoq.Template.All.
 Require Import Coq.Lists.List.
+Require Import Coq.Program.Wf.
+Require Import Coq.micromega.Lia.
 Import String.
 
 Import MCMonadNotation.
 Import ListNotations.
 Open Scope bs.
+
+Require Import MirrorSolve.Reflection.Meta.
 
 Definition tmDebug {A: Type} (thing: A) : TemplateMonad unit :=
   tmEval all thing >>= tmPrint
@@ -38,16 +42,16 @@ Fixpoint inspect_ctor_args
     | first_body :: nil =>
       match nth_error first_body.(ind_ctors) index with
       | Some inductive_ctor =>
-        tmReturn (List.length inductive_ctor.(cstr_args), nil)
+        tmReturn (List.length inductive_ctor.(cstr_args), 0)
       | None =>
         tmFail "Inductive constructor out of range"
       end
     | _ =>
       tmFail "Inductive has more than one body."
     end
-  | tApp ind_term args =>
-    mlet '(arg_count, type_args) <- inspect_ctor_args ind_term index ;;
-    tmReturn (arg_count, args ++ type_args)%list
+  | tApp ind_term inst_args =>
+    mlet '(arg_count, inst_arg_count) <- inspect_ctor_args ind_term index ;;
+    tmReturn (arg_count, inst_arg_count + #|inst_args|)%list
   | _ =>
     tmDebug ind_term ;;
     tmFail "Term is not an inductive."
@@ -126,103 +130,395 @@ Fixpoint subst_nolift (s : list term) (k : nat) (u : term) : term :=
 Definition infer_equation
   (arg_type_quoted: term)
   (ret_type_quoted: term)
-  (func_quoted: term)
+  (func_ref: kername * Instance.t)
   (info: case_info)
   (body: term)
   (depth: nat)
   (offset: nat)
   (index: nat)
 :=
-  mlet (arg_count, inst_args) <- inspect_ctor_args arg_type_quoted index ;;
-  match func_quoted with
-  | tConst (_, func_name) _ =>
-    let construct := tApp (tConstruct info.(ci_ind) index [])
-                          (inst_args ++ dummy_args arg_count 0)%list in
-    let args_pre := dummy_args (depth-1-offset) (offset+arg_count) in
-    let args_post := dummy_args offset arg_count in
-    let args := (args_pre ++ [construct] ++ args_post)%list in
-    let claim_lhs := tApp func_quoted args in
-    let claim_rhs := subst_nolift [construct] (offset+arg_count) body in
-    let (claim_prefix, proof_prefix) :=
-      match ret_type_quoted with
-      | tSort Universe.lProp =>
-        (iff_quoted, iff_refl_quoted)
-      | _ =>
-        (tApp eq_quoted [hole], tApp eq_refl_quoted [hole])
-      end in
-    let claim_eq := tApp claim_prefix [claim_lhs; claim_rhs] in
-    let claim_quoted := wrap_type (arg_count+depth-1) claim_eq in
-    claim <- tmUnquoteTyped Type claim_quoted ;;
-    let proof_quoted :=
-      wrap_body (arg_count+depth-1) (tApp proof_prefix [claim_rhs]) in
-    proof <- tmUnquoteTyped claim proof_quoted ;;
-    let eqn_base := func_name ++ "_equation_" ++ string_of_nat (index+1) in
-    eqn_name <- tmFreshName eqn_base ;;
-    tmDefinitionRed eqn_name (Some (unfold (Common_kn "my_projT1"))) proof ;;
-    tmReturn tt
-  | _ => tmFail "Symbol is not a constant."
-  end
+  mlet (arg_count, inst_arg_count) <- inspect_ctor_args arg_type_quoted index ;;
+  let (func_kername, func_inst) := func_ref in
+  let (func_path, func_name) := func_kername in
+  let construct := tApp (tConstruct info.(ci_ind) index [])
+                        (repeat hole inst_arg_count
+                         ++ dummy_args arg_count 0)%list in
+  let args_pre := dummy_args (depth-1-offset) (offset+arg_count) in
+  let args_post := dummy_args offset arg_count in
+  let args := (args_pre ++ [construct] ++ args_post)%list in
+  let claim_lhs := tApp (tConst func_kername func_inst) args in
+  let claim_rhs := subst_nolift [construct] (offset+arg_count) body in
+  let (claim_prefix, proof_prefix) :=
+    match ret_type_quoted with
+    | tSort Universe.lProp =>
+      (iff_quoted, iff_refl_quoted)
+    | _ =>
+      (tApp eq_quoted [hole], tApp eq_refl_quoted [hole])
+    end in
+  let claim_eq := tApp claim_prefix [claim_lhs; claim_rhs] in
+  let claim_quoted := wrap_type (arg_count+depth-1) claim_eq in
+  claim <- tmUnquoteTyped Type claim_quoted ;;
+  let proof_quoted :=
+    wrap_body (arg_count+depth-1) (tApp proof_prefix [claim_rhs]) in
+  proof <- tmUnquoteTyped claim proof_quoted ;;
+  let eqn_base := func_name ++ "_equation_" ++ string_of_nat (index+1) in
+  eqn_name <- tmFreshName eqn_base ;;
+  tmDefinitionRed eqn_name (Some (unfold (Common_kn "my_projT1"))) proof ;;
+  tmReturn tt
 .
 
 Fixpoint infer_equations_walk_cases
   (arg_type_quoted: term)
   (ret_type_quoted: term)
-  (func_quoted: term)
+  (func_ref: kername * Instance.t)
   (info: case_info)
   (bodies: list (branch term))
   (depth: nat)
   (offset: nat)
   (index: nat)
+:
+  TemplateMonad unit
 :=
   match bodies with
-  | nil => tmReturn 0
+  | nil => tmReturn tt
   | body :: bodies =>
-    infer_equation arg_type_quoted ret_type_quoted func_quoted info body.(bbody) depth offset index ;;
-    infer_equations_walk_cases arg_type_quoted ret_type_quoted func_quoted info bodies depth offset (S index)
+    infer_equation arg_type_quoted ret_type_quoted func_ref info body.(bbody) depth offset index ;;
+    infer_equations_walk_cases arg_type_quoted ret_type_quoted func_ref info bodies depth offset (S index)
   end
 .
 
-Fixpoint infer_equations_inner
+Fixpoint term_lambda_depth (u : term) : nat :=
+  match u with
+  | tEvar _ args =>
+    list_max (map term_lambda_depth args)
+  | tCast c _ ty =>
+    max (term_lambda_depth c) (term_lambda_depth ty)
+  | tProd _ A B =>
+    max (term_lambda_depth A) (term_lambda_depth B)
+  | tLambda _ T M =>
+    max (term_lambda_depth T) (S (term_lambda_depth M))
+  | tLetIn _ b ty b' =>
+    list_max [
+      term_lambda_depth b;
+      term_lambda_depth ty;
+      term_lambda_depth b'
+    ]
+  | tApp u0 v =>
+    list_max (map term_lambda_depth (u0 :: v))
+  | tCase _ p c brs =>
+    list_max (map term_lambda_depth p.(pparams)
+             ++ [term_lambda_depth p.(preturn)]
+             ++ [term_lambda_depth c]
+             ++ map (term_lambda_depth ∘ bbody) brs)
+  | tProj _ c =>
+    term_lambda_depth c
+  | tFix mfix _
+  | tCoFix mfix _ =>
+    list_max (map (term_lambda_depth ∘ dtype) mfix
+              ++ map (S ∘ term_lambda_depth ∘ dbody) mfix)
+  | _ => 0
+  end
+.
+
+Lemma term_lambda_depth_lift (t: term) (n m: nat):
+  term_lambda_depth (lift n m t) = term_lambda_depth t
+.
+Proof.
+  revert n m; induction t using term_ind'; intros; simpl; try congruence.
+  - rewrite Forall_forall in H.
+    rewrite map_map.
+    now erewrite map_ext_in.
+  - rewrite Forall_forall in H.
+    f_equal; auto.
+    rewrite map_map.
+    now erewrite map_ext_in.
+  - rewrite Forall_forall in H, H0.
+    f_equal; f_equal; [| f_equal; [| f_equal]].
+    + now erewrite map_map, map_ext_in.
+    + now rewrite IHt.
+    + now rewrite IHt0.
+    + erewrite map_map, map_ext_in; intuition.
+  - rewrite Forall_forall in H, H0.
+    f_equal; f_equal; erewrite map_map, map_ext_in; intuition.
+  - rewrite Forall_forall in H, H0.
+    f_equal; f_equal; erewrite map_map, map_ext_in; intuition.
+Qed.
+
+Lemma term_lambda_depth_mkApps (t: term) (args: list term):
+  term_lambda_depth (mkApps t args) = term_lambda_depth (tApp t args)
+.
+Proof.
+  destruct args; simpl.
+  - lia.
+  - destruct t; simpl; try lia.
+    rewrite map_app, list_max_app.
+    simpl; lia.
+Qed.
+
+Lemma list_max_In (l: list nat) (n: nat):
+  In n l ->
+  n <= list_max l
+.
+Proof.
+  induction l; intros; destruct H; simpl.
+  - lia.
+  - etransitivity; swap 1 2.
+    + apply PeanoNat.Nat.le_max_r.
+    + intuition.
+Qed.
+
+Lemma list_max_add_distr_l (l: list nat) (n: nat):
+  l <> nil ->
+  n + list_max l = list_max (map (Nat.add n) l)
+.
+Proof.
+  induction l; simpl; intros.
+  - contradiction.
+  - destruct l.
+    + simpl; lia.
+    + rewrite PeanoNat.Nat.max_comm.
+      rewrite <- IHl.
+      * lia.
+      * intro.
+        discriminate.
+Qed.
+
+Lemma term_lambda_depth_subst1 (t u: term) (n: nat):
+  term_lambda_depth (subst [t] n u) <= term_lambda_depth t + term_lambda_depth u
+.
+Proof.
+  revert n; induction u using term_ind'; intros; simpl; try lia.
+  - destruct (PeanoNat.Nat.leb _ _).
+    + destruct (n - n0); simpl.
+      * now rewrite term_lambda_depth_lift.
+      * rewrite nth_error_nil; simpl; lia.
+    + now simpl.
+  - apply list_max_le.
+    rewrite Forall_forall; intros.
+    rewrite Forall_forall in H.
+    rewrite map_map in H0.
+    apply in_map_iff in H0.
+    destruct H0 as [t' [? ?]]; subst.
+    etransitivity.
+    + now apply H.
+    + apply PeanoNat.Nat.add_le_mono_l.
+      apply list_max_In.
+      apply in_map_iff.
+      now exists t'.
+  - specialize (IHu1 n).
+    specialize (IHu2 n).
+    lia.
+  - specialize (IHu1 n).
+    specialize (IHu2 (S n)).
+    lia.
+  - specialize (IHu1 n).
+    specialize (IHu2 (S n)).
+    lia.
+  - specialize (IHu1 n).
+    specialize (IHu2 n).
+    specialize (IHu3 (S n)).
+    lia.
+  - rewrite term_lambda_depth_mkApps; simpl.
+    rewrite Forall_forall in H.
+    rewrite <- Max.plus_max_distr_l.
+    apply Max.max_lub.
+    + specialize (IHu n); lia.
+    + apply list_max_le.
+      apply Forall_forall; intros.
+      rewrite map_map in H0.
+      apply in_map_iff in H0.
+      destruct H0 as [t' [? ?]]; subst.
+      rewrite <- PeanoNat.Nat.le_max_r.
+      rewrite list_max_add_distr_l.
+      * rewrite map_map.
+        rewrite H by auto.
+        apply list_max_In.
+        apply in_map_iff.
+        eexists; auto.
+      * intro.
+        apply map_eq_nil in H0; now subst.
+  - rewrite list_max_add_distr_l.
+    + repeat rewrite map_app.
+      repeat rewrite map_map.
+      rewrite Forall_forall in H, H0.
+      apply list_max_le, Forall_forall; intros.
+      apply in_app_iff in H1; simpl in H1.
+      repeat rewrite list_max_app; simpl.
+      destruct H1 as [? | [? | [? | ?]]]; subst.
+      * apply in_map_iff in H1.
+        destruct H1 as [t' [? ?]]; subst.
+        rewrite <- PeanoNat.Nat.le_max_l.
+        etransitivity; swap 1 2.
+        apply list_max_In.
+        apply in_map_iff.
+        now exists t'.
+        now apply H.
+      * specialize (IHu (#|pcontext type_info| + n)); lia.
+      * specialize (IHu0 n); lia.
+      * repeat rewrite <- PeanoNat.Nat.le_max_r.
+        rewrite map_map.
+        apply in_map_iff in H1.
+        destruct H1 as [? [? ?]]; subst.
+        etransitivity; [now apply H0|].
+        apply list_max_In.
+        apply in_map_iff.
+        now eexists.
+    + intro.
+      apply (f_equal (@List.length nat)) in H1.
+      rewrite app_length in H1; simpl in H1.
+      lia.
+  - apply IHu.
+  - apply list_max_le, Forall_forall; intros.
+    rewrite in_app_iff in H1.
+    rewrite list_max_add_distr_l.
+    + repeat rewrite in_map_iff in H1.
+      destruct H1.
+      * destruct H1 as [? [? ?]]; subst.
+        apply in_map_iff in H2.
+        destruct H2 as [? [? ?]]; subst.
+        rewrite <- map_dtype.
+        rewrite map_app, list_max_app.
+        rewrite Forall_forall in H.
+        rewrite H by auto.
+        rewrite <- PeanoNat.Nat.le_max_l.
+        rewrite map_map.
+        apply list_max_In.
+        apply in_map_iff.
+        now eexists.
+      * destruct H1 as [? [? ?]]; subst.
+        apply in_map_iff in H2.
+        destruct H2 as [? [? ?]]; subst.
+        rewrite <- map_dbody.
+        rewrite map_app, list_max_app.
+        rewrite Forall_forall in H0.
+        rewrite <- PeanoNat.Nat.le_max_r.
+        etransitivity; swap 1 2.
+        rewrite map_map.
+        apply list_max_In.
+        apply in_map_iff.
+        now eexists.
+        specialize (H0 _ H2 (#|mfix| + n)).
+        lia.
+    + intro.
+      apply (f_equal (@List.length nat)) in H2.
+      rewrite app_length in H2; simpl in H2.
+      repeat rewrite map_length in H2.
+      apply Plus.plus_is_O in H2.
+      destruct H2 as [? _].
+      apply length_zero_iff_nil in H2.
+      destruct H1.
+      * rewrite map_map in H1.
+        rewrite in_map_iff in H1.
+        destruct H1 as [? [? ?]].
+        now subst.
+      * rewrite map_map in H1.
+        rewrite in_map_iff in H1.
+        destruct H1 as [? [? ?]].
+        now subst.
+  - apply list_max_le, Forall_forall; intros.
+    rewrite in_app_iff in H1.
+    rewrite list_max_add_distr_l.
+    + repeat rewrite in_map_iff in H1.
+      destruct H1.
+      * destruct H1 as [? [? ?]]; subst.
+        apply in_map_iff in H2.
+        destruct H2 as [? [? ?]]; subst.
+        rewrite <- map_dtype.
+        rewrite map_app, list_max_app.
+        rewrite Forall_forall in H.
+        rewrite H by auto.
+        rewrite <- PeanoNat.Nat.le_max_l.
+        rewrite map_map.
+        apply list_max_In.
+        apply in_map_iff.
+        now eexists.
+      * destruct H1 as [? [? ?]]; subst.
+        apply in_map_iff in H2.
+        destruct H2 as [? [? ?]]; subst.
+        rewrite <- map_dbody.
+        rewrite map_app, list_max_app.
+        rewrite Forall_forall in H0.
+        rewrite <- PeanoNat.Nat.le_max_r.
+        etransitivity; swap 1 2.
+        rewrite map_map.
+        apply list_max_In.
+        apply in_map_iff.
+        now eexists.
+        specialize (H0 _ H2 (#|mfix| + n)).
+        lia.
+    + intro.
+      apply (f_equal (@List.length nat)) in H2.
+      rewrite app_length in H2; simpl in H2.
+      repeat rewrite map_length in H2.
+      apply Plus.plus_is_O in H2.
+      destruct H2 as [? _].
+      apply length_zero_iff_nil in H2.
+      destruct H1.
+      * rewrite map_map in H1.
+        rewrite in_map_iff in H1.
+        destruct H1 as [? [? ?]].
+        now subst.
+      * rewrite map_map in H1.
+        rewrite in_map_iff in H1.
+        destruct H1 as [? [? ?]].
+        now subst.
+Qed.
+
+Polymorphic Program Fixpoint infer_equations_inner
   (body: term)
-  (top_quoted: term)
+  (func_ref: kername * Instance.t)
   (context: list term)
+  {measure (term_lambda_depth body)}
+:
+  TemplateMonad unit
 :=
   match body with
   | tLambda _ arg_type_quoted body =>
-    infer_equations_inner body top_quoted (arg_type_quoted :: context)
+    infer_equations_inner body func_ref (arg_type_quoted :: context)
   | tCase info pred (tRel offset) bodies =>
     match nth_error context offset with
     | Some arg_type_quoted =>
-      infer_equations_walk_cases arg_type_quoted pred.(preturn) top_quoted info bodies (List.length context) offset 0
+      infer_equations_walk_cases arg_type_quoted pred.(preturn) func_ref info bodies (List.length context) offset 0
     | None =>
       tmFail "Term contains match on something that is not an argument."
     end
+  | tFix (first_fixpoint :: nil) 0 =>
+    let rec_call := tApp (uncurry tConst func_ref) (dummy_args #|context| 0) in
+    let body := subst10 rec_call first_fixpoint.(dbody) in
+    infer_equations_inner body func_ref context
   | _ =>
     tmFail "Symbol body is not a function with a match inside."
   end
 .
-
-Definition infer_equations_handle_fixpoint
-  (body: term)
-  (func_quoted: term)
-:=
-  match body with
-  | tFix (first_fixpoint :: nil) 0 =>
-    let body := subst10 func_quoted first_fixpoint.(dbody) in
-    infer_equations_inner body func_quoted nil
-  | _ =>
-    infer_equations_inner body func_quoted nil
-  end
-.
+Next Obligation.
+  simpl; lia.
+Qed.
+Next Obligation.
+  simpl.
+  eapply PeanoNat.Nat.le_lt_trans.
+  - apply term_lambda_depth_subst1.
+  - simpl.
+    eapply PeanoNat.Nat.le_lt_trans.
+    + apply PeanoNat.Nat.add_le_mono_r.
+      instantiate (1 := 0).
+      generalize 0 at 1; induction context0; simpl; intros.
+      * lia.
+      * rewrite map_app; simpl.
+        rewrite list_max_app; simpl.
+        rewrite PeanoNat.Nat.max_0_r.
+        apply IHcontext0.
+    + lia.
+Qed.
+Solve Obligations with (repeat split; intros; intro; discriminate).
 
 Definition infer_equations {A: Type} (func: A) :=
   func_quoted <- tmQuote func ;;
   match func_quoted with
-  | tConst func_path _ =>
+  | tConst func_path func_inst =>
     def <- tmQuoteConstant func_path true ;;
     match def.(cst_body) with
     | Some body =>
-      infer_equations_handle_fixpoint body func_quoted
+      infer_equations_inner body (func_path, func_inst) nil
     | None =>
       tmFail "Function does not seem to have a body."
     end
@@ -292,12 +588,6 @@ Section Tests.
   Check mul_equation_1.
   Check mul_equation_2.
 
-  Definition app_nat := Eval compute in (@List.app nat).
-
-  MetaCoq Run (infer_equations app_nat).
-  Check app_nat_equation_1.
-  Check app_nat_equation_2.
-
   Fixpoint NoDup_nat (xs: list nat) :=
     match xs with
     | [] => True
@@ -307,4 +597,12 @@ Section Tests.
   MetaCoq Run (infer_equations NoDup_nat).
   Check NoDup_nat_equation_1.
   Check NoDup_nat_equation_2.
+
+  MetaCoq Run (infer_equations List.app).
+  Check app_equation_1.
+  Check app_equation_2.
+
+  MetaCoq Run (infer_equations List.rev).
+  Check rev_equation_1.
+  Check rev_equation_2.
 End Tests.
